Refactor ErrorWithWriter; Finish bool_decoder vst spec

src/PrimitiveDecoder/ErrorWithWriter.v
@@ -8,11 +8,11 @@ Open Scope monad.
 
 Section Error.
 
+Context {E : Type}.
 Context {T : Type}.
-Context {Wr : Type}.
-Context {MWr : Monoid Wr}.
+Context {MT : Monoid T}.
 
-Definition errW A := Wr -> T + (Wr * A).
+Definition errW A := T -> E + (T * A).
 
 Global Instance Monad_errW : Monad errW := {
   ret := fun _ x => fun w => inr (w, x) ;
@@ -22,7 +22,7 @@ Global Instance Monad_errW : Monad errW := {
                             end
 }.
 
-Global Instance Exception_errW : MonadExc T errW := {
+Global Instance Exception_errW : MonadExc E errW := {
   raise := fun _ v => fun w => inl v ;
   catch := fun _ c h => fun w => match c w with
                            | inl v => h v w
@@ -30,7 +30,7 @@ Global Instance Exception_errW : MonadExc T errW := {
                            end
 }.
 
-Global Instance Writer_errW : MonadWriter MWr errW := {
+Global Instance Writer_errW : MonadWriter MT errW := {
   tell := fun w => fun _ => inr (w, tt) ;
   listen := fun _ m => fun w => match m w with 
                           | inl v => inl v 
@@ -42,13 +42,13 @@ Global Instance Writer_errW : MonadWriter MWr errW := {
                         end ;
 }.
 
-Definition evalErrW {A : Type} (e : errW A) (init : Wr) : option A := 
+Definition evalErrW {A : Type} (e : errW A) (init : T) : option A := 
   match e init with
   | inl _ => None
   | inr (_, v) => Some v
   end.
 
-Definition execErrW {A : Type} (e : errW A) (init : Wr) : option Wr :=
+Definition execErrW {A : Type} (e : errW A) (init : T) : option T :=
   match e init with
   | inl _ => None
   | inr (w, _) => Some w
