src/PrimitiveDecoder/BooleanVSTSpec.v
@@ -79,67 +79,67 @@ Section Boolean_der_decode_primitive.
 
 Definition bool_ber_decode_spec : ident * funspec :=
   DECLARE _BOOLEAN_decode_ber
-    WITH (* pointer to the decoded structure *)
-         sptr_b : block, sptr_ofs : ptrofs,
-         (* double pointer to the DEF table for the type decoded *)
-         td_b : block, td_ofs : ptrofs,
-         td'_b : block, td'_ofs : ptrofs,
-         (* pointer to  the input buffer *)
-         buf_b : block, buf_ofs : ptrofs,
-         (* pointer to the return struct dec_rval *)                         
-         res_b : block, res_ofs : ptrofs,
-         (* codec context: stores max_stack_size for the decoder routines *)
-         ctx : val,
-         (* memory permissions for each pointer *)
-         sh_sptr : share, sh_td : share, sh_buf : share, sh_td' : share,
-         sh_res : share,                                                         
-         (* input *)
-         buf : list byte,
-         td : TYPE_descriptor,
-         size : int,
-         tag_mode : int  
+    WITH (* Context pointer *)
+         sh_ctx : share, ctx_b : block, ctx_ofs : ptrofs, ctx : val,
+         (* Type Descriptor pointer *)
+         sh_td : share, td_b : block, td_ofs : ptrofs, td : TYPE_descriptor,
+         (* Value double pointer *)
+         sh_val' : share, val_b' : block, val_ofs' : ptrofs,
+         sh_val : share, val_b : block, val_ofs : ptrofs,
+         (* Buffer pointer *)
+         sh_buf : share, buf_b : block, buf_ofs : ptrofs, buf : list byte,
+         size : Z, tag_mode : Z
     PRE  [         
- (* added by clightgen - since returning structs is not supported *) 
-          __res OF (tptr (Tstruct _asn_dec_rval_s noattr)),
-          _opt_codec_ctx OF (tptr (Tstruct _asn_codec_ctx_s noattr)),
-          _td OF (tptr (Tstruct _asn_TYPE_descriptor_s noattr)),
-          _sptr OF (tptr (tptr tvoid)),
-          _buf_ptr OF (tptr tvoid),
-          _size OF tuint,
-          _tag_mode OF tint ]
-    PROP ( writable_share sh_sptr; 
-           writable_share sh_res; 
-           readable_share sh_td;
+         (* added by clightgen - since returning structs is not supported *) 
+         __res OF (tptr (Tstruct _asn_dec_rval_s noattr)),
+         _opt_codec_ctx OF (tptr (Tstruct _asn_codec_ctx_s noattr)),
+         _td OF (tptr (Tstruct _asn_TYPE_descriptor_s noattr)),
+         _bool_value OF (tptr (tptr tvoid)),
+         _buf_ptr OF (tptr tvoid),
+         _size OF tuint,
+         _tag_mode OF tint]
+    PROP ( readable_share sh_ctx; 
+           readable_share sh_td; 
+           readable_share sh_val';
+           readable_share sh_val;
            readable_share sh_buf )
     LOCAL ( temp _opt_codec_ctx ctx;
             temp _td (Vptr td_b td_ofs);
-            temp _sptr (Vptr sptr_b sptr_ofs);
+            temp _bool_value (Vptr val_b' val_ofs');
             temp _buf_ptr (Vptr buf_b buf_ofs);
-            temp _size (Vint size);
-            temp _tag_mode (Vint tag_mode))        
-    SEP ((* td points to td with readable permission *)
-           data_at sh_td (tptr (Tstruct _asn_TYPE_descriptor_s noattr)) 
-                   (Vptr td'_b td'_ofs) (Vptr td_b td_ofs);
-           data_at sh_td' (Tstruct _asn_TYPE_descriptor_s noattr) 
-                   (TYPE_descriptor_rep td) (Vptr td'_b td'_ofs) ; 
+            temp _size (Vint (Int.repr size));
+            temp _tag_mode (Vint (Int.repr tag_mode)))
+    SEP (
+           data_at sh_ctx (tptr (Tstruct _asn_codec_ctx_s noattr))
+                   (Vptr ctx_b ctx_ofs) (ctx);
+           data_at sh_td (Tstruct _asn_TYPE_descriptor_s noattr)
+                   (TYPE_descriptor_rep td) (Vptr td_b td_ofs);
+           (* val double pointer *)
+           data_at sh_val' (tptr (tptr tuchar)) (Vptr val_b val_ofs)
+                   (Vptr val_b' val_ofs');
+           data_at sh_val (tptr tuchar) (default_val (tptr tuchar)) (Vptr val_b val_ofs);
            (* buf points to data ls *)
            data_at sh_buf (tarray tschar (Zlength buf)) (map Vbyte buf) 
                    (Vptr buf_b buf_ofs))
     POST [tvoid]
       PROP()
       LOCAL ()
-      SEP( (* Unchanged by the execution : *)
-           data_at sh_td (tptr (Tstruct _asn_TYPE_descriptor_s noattr)) 
-                   (Vptr td'_b td'_ofs) (Vptr td_b td_ofs);
-           data_at sh_td' (Tstruct _asn_TYPE_descriptor_s noattr) 
-                   (TYPE_descriptor_rep td) (Vptr td'_b td'_ofs) ; 
+      SEP( 
+           (* Unchanged by the execution : *)
+           data_at sh_ctx (tptr (Tstruct _asn_codec_ctx_s noattr))
+                   (Vptr ctx_b ctx_ofs) (ctx);
+           data_at sh_td (Tstruct _asn_TYPE_descriptor_s noattr) 
+                   (TYPE_descriptor_rep td) (Vptr td_b td_ofs);
            data_at sh_buf (tarray tschar (Zlength buf)) (map Vbyte buf) 
                    (Vptr buf_b buf_ofs);
-           (* Changed after execution *)         
-           data_at sh_sptr (Tstruct _asn_TYPE_descriptor_s noattr) 
-                   (bool_prim_decoder td buf) (Vptr sptr_b sptr_ofs); 
-           data_at sh_res (Tstruct _asn_dec_rval_s noattr)
-                   (dec_rval_rep (bool_prim_decoder td buf)) (Vptr res_b res_ofs)).
+           data_at sh_val' (tptr (tptr tuchar)) (Vptr val_b val_ofs) 
+                   (Vptr val_b' val_ofs');
+           (* Changed after execution *)
+           let res := bool_decoder td buf in
+           match res with
+           | Some r => data_at sh_val (tptr tuchar) (Vbyte r) (Vptr val_b val_ofs)
+           | None => data_at sh_val (tptr tuchar) (default_val (tptr tuchar)) (Vptr val_b val_ofs)
+           end).
 
 Definition Gprog2 := ltac:(with_library prog [bool_ber_decode_spec]).
 
